Expose that array length fits in a size_t

pulse/ulib/experimental/Steel.ST.Array.fst
@@ -88,6 +88,7 @@ let ptr elt = H.ptr (raise_t elt)
 let base p = H.base p
 let offset p = H.offset p
 let ptr_base_offset_inj p1 p2 = H.ptr_base_offset_inj p1 p2
+let length_fits a = H.length_fits a
 
 let pts_to a p s = H.pts_to a p (seq_map raise s)
 
